Rename multiply copy

src/verification/stream_multiply.lean
@@ -1,905 +1,161 @@
 import tactic
 import data.finsupp.basic
 import control.bifunctor
-import verification.vars
-import verification.verify
 import verification.misc
+import verification.stream_props
 
 open_locale classical
 noncomputable theory
 
-variables {σ α ι β ρ : Type}
-variables (R : Type) [add_zero_class R] [has_one R] [has_mul R]
-
-variables
+variables {σ₁ σ₂ α ι : Type}
 [linear_order ι]
-
-structure partial_status (σ ι α : Type) :=
-(index : with_top ι)
-(value : option α)
-(ready : bool)
-(valid : bool)
-(state : σ)
-
-@[reducible, inline]
-def StreamState.valid (s : StreamState σ ι α) : Prop := s.stream.valid s.state
-@[reducible, inline]
-def StreamState.ready (s : StreamState σ ι α) : Prop := s.stream.ready s.state
-
-def StreamState.now' (s : StreamState σ ι ρ) : partial_status σ ι ρ :=
-{ index := if h : s.stream.valid s.state then s.stream.index s.state h else ⊤,
-  value := if h : s.stream.ready s.state then s.stream.value s.state h else none,
-  ready := s.stream.ready s.state,
-  valid := s.stream.valid s.state,
-  state := s.state }
-
-@[simp]
-def StreamExec.now' (s : StreamExec σ ι ρ) : partial_status σ ι ρ :=
-s.to_StreamState.now'
-
-open Types
-
-open Stream StreamExec
-
-@[reducible] def stream_order_tuple (ι : Type) : Type := bool ×ₗ with_top ι ×ₗ bool
-example : linear_order (stream_order_tuple ι) := infer_instance
-
-def StreamState.to_order_tuple {α} (a : StreamState σ ι α) : stream_order_tuple ι :=
-(¬ a.now'.valid, a.now'.index, a.now'.ready)
---let a := p.1, s := p.2 in (¬ a.valid s, if h : a.valid s then a.index s h else ⊤, a.ready s)
-def StreamExec.to_order_tuple {α} (a : StreamExec σ ι α) : bool ×ₗ with_top ι ×ₗ bool :=
-a.to_StreamState.to_order_tuple
-
-variables {σ₁ σ₂ : Type}
-
-def StreamState.lag {σ₁ σ₂ ι α β} [linear_order ι] : StreamState σ₁ ι α → StreamState σ₂ ι β → Prop := λ a b, a.to_order_tuple ≤ b.to_order_tuple
-def StreamState.lag_lt {α β} : StreamState σ₁ ι α → StreamState σ₂ ι β → Prop := λ a b, a.to_order_tuple < b.to_order_tuple
-def StreamExec.lag  {α β} : StreamExec σ₁ ι α → StreamExec σ₂ ι β → Prop := λ a b, a.to_order_tuple ≤ b.to_order_tuple
-def StreamExec.lag_lt  {α β} : StreamExec σ₁ ι α → StreamExec σ₂ ι β → Prop := λ a b, a.to_order_tuple < b.to_order_tuple
-
-instance (σ ι α : Type) : has_coe (StreamExec σ ι α) (StreamState σ ι α) := ⟨StreamExec.to_StreamState⟩
-
-instance StreamState.preorder : preorder (StreamState σ ι α) := preorder.lift StreamState.to_order_tuple
-instance StreamExec.preorder : preorder (StreamExec σ ι α) := preorder.lift StreamExec.to_order_tuple
-
-local infix `⊑`:50    := StreamExec.lag
-local infix `⊏`:50    := StreamExec.lag_lt
-local infix `⊑ₛ`:50   := StreamState.lag
-local infix `⊏ₛ`:50   := StreamState.lag_lt
-
-lemma StreamExec.le_total {α β : Type} (a : StreamExec σ₁ ι α) (b : StreamExec σ₂ ι β) : a.lag b ∨ b.lag a := le_total a.to_order_tuple b.to_order_tuple
-
-def Stream.monotonic (q : Stream σ ι α) : Prop :=
-∀ {r} (h : q.valid r), StreamState.lag ⟨q, r⟩ ⟨q, q.next r h⟩
-
-def Stream.reduced (q : Stream σ ι α) : Prop :=
-∀ {s t} (hs : q.valid s) (ht : q.valid t), q.ready s → q.ready t → q.index s hs = q.index t ht → s = t
-
-variables {σ ι α}
-
-variables
-(s : StreamExec σ ι α)
-(a : StreamExec σ₁ ι α)
-(b : StreamExec σ₂ ι α)
-(s₁ : σ₁) (s₂ : σ₂)
-[non_unital_semiring α]
-
--- no assumptions on value type
-variables (q : StreamExec σ ι ρ)
-
-@[simp] lemma StreamExec.bound_valid_zero' {s : StreamExec σ ι α} :
-  s.bound = 0 → (s.bound_valid ↔ ¬s.valid) := λ bz,
-by simp [StreamExec.bound_valid, bz]
+[non_unital_non_assoc_semiring α]
 
 @[mk_iff]
 structure Stream.mul.ready (a : Stream σ₁ ι α) (b : Stream σ₂ ι α) (s : σ₁ × σ₂) : Prop :=
-(valid : a.valid s.1 ∧ b.valid s.2)
-(ready : a.ready s.1 ∧ b.ready s.2)
-(index : a.index s.1 valid.1 = b.index s.2 valid.2)
+(v₁ : a.valid s.1)
+(v₂ : b.valid s.2)
+(r₁ : a.ready s.1)
+(r₂ : b.ready s.2)
+(index : a.index s.1 v₁ = b.index s.2 v₂)
 
 @[simps]
-def Stream.mul {σ₁ σ₂} (a : Stream σ₁ ι α) (b : Stream σ₂ ι α) : Stream (σ₁ × σ₂) ι α :=
+def Stream.mul (a : Stream σ₁ ι α) (b : Stream σ₂ ι α) : Stream (σ₁ × σ₂) ι α :=
 { valid := λ p, a.valid p.1 ∧ b.valid p.2,
   ready := λ p, Stream.mul.ready a b p,
-  next  := λ p hv, if StreamState.lag ⟨a, p.1⟩ ⟨b, p.2⟩ then (a.next p.1 hv.1, p.2) else (p.1, b.next p.2 hv.2),
+  next  := λ p hv, if a.to_order p.1 ≤ b.to_order p.2 then (a.next p.1 hv.1, p.2) else (p.1, b.next p.2 hv.2),
   index := λ p hv, max (a.index p.1 hv.1) (b.index p.2 hv.2),
-  value := λ p hr, a.value p.1 hr.ready.1 * b.value p.2 hr.ready.2 }
+  value := λ p hr, a.value p.1 hr.r₁ * b.value p.2 hr.r₂ }
+
+infixl ` ⋆ `:71 := Stream.mul
+
+section lemmas
+
+lemma Stream.mul.eq_order_of_ready {a : Stream σ₁ ι α} {b : Stream σ₂ ι α} {x y} (h : (a ⋆ b).ready (x, y)) :
+  a.to_order x = b.to_order y :=
+by ext : 1; simp [h.r₁, h.r₂, Stream.index'_val h.v₁, Stream.index'_val h.v₂, h.index]
+
+lemma Stream.mul_eval₀_of_neq {a : Stream σ₁ ι α} {b : Stream σ₂ ι α} {x y} (h : a.to_order x ≠ b.to_order y) (H) :
+  (a ⋆ b).eval₀ (x, y) H = 0 :=
+by { contrapose! h, apply Stream.mul.eq_order_of_ready, simp [Stream.eval₀] at h, exact h.fst, }
+
+lemma Stream.mul_eval₀ (a : Stream σ₁ ι α) (b : Stream σ₂ ι α) (x : σ₁) (y : σ₂) (H) :
+  (a ⋆ b).eval₀ (x, y) H = (a.eval₀ x H.1) * (b.eval₀ y H.2) :=
+begin
+  rw [Stream.eval₀], split_ifs with hr,
+  { simp [Stream.eval₀, hr.r₁, hr.r₂, hr.index], },
+  simp [Stream.mul.ready_iff, H.1, H.2] at hr,
+  simp [Stream.eval₀], split_ifs with h₁ h₂; try { simp },
+  rw finsupp.mul_single_eq_zero _ _ (hr h₁ h₂),
+end
+
+/-- This lemma states that if `a.to_order x ≤ b.to_order y`, 
+  then the support of `a.eval₀ x h₁` (which is at most `{a.index x}`) 
+  is disjoint from `b.eval_steps n (b.next y)`, assuming `b` is simple. -/
+lemma Stream.mul_eq_zero_aux {a : Stream σ₁ ι α} {b : Stream σ₂ ι α} [b.simple] {x : σ₁} {y : σ₂}
+  (h₁ : a.valid x) (h₂ : b.valid y) (H : a.to_order x ≤ b.to_order y) (n : ℕ) :
+  disjoint (a.eval₀ x h₁).support (b.eval_steps n (b.next y h₂)).support :=
+begin
+  -- Assume `a` is ready, or else `a.eval₀ x h₁ = 0` has trivial support.
+  by_cases hr : a.ready x, swap, { simp [Stream.eval₀, hr], },
+  rw finset.disjoint_iff_ne,
+  intros i₁ hi₁ i₂ hi₂,
+  cases finset.mem_singleton.mp (a.eval₀_support _ _ hi₁),
+  rw le_iff_eq_or_lt at H,
+  refine ne_of_lt (with_top.coe_lt_coe.mp _), rw ← Stream.index'_val h₁,
+  cases H,
+  { -- `a.to_order x = b.to_order y`
+    simp [prod.ext_iff, hr] at H,
+    rw H.1,
+    exact b.index_lt_support h₂ H.2 _ hi₂, },
+  -- Case `a < b`
+  refine lt_of_lt_of_le (prod.lex.fst_lt_of_lt_of_le H (by simp [hr])) _,
+  exact (b.is_monotonic h₂).trans (b.is_monotonic.index_le_support _ hi₂),
+end
+
+lemma Stream.mul_eq_zero {a : Stream σ₁ ι α} {b : Stream σ₂ ι α} [b.simple] {x : σ₁} {y : σ₂}
+  (h₁ : a.valid x) (h₂ : b.valid y) (H : a.to_order x ≤ b.to_order y) (n : ℕ) :
+  a.eval₀ x h₁ * b.eval_steps n (b.next y h₂) = 0 :=
+by { rw [finsupp.mul_eq_zero_of_disjoint_support], exact Stream.mul_eq_zero_aux h₁ h₂ H n, }
+
+lemma Stream.mul_eq_zero' {a : Stream σ₁ ι α} {b : Stream σ₂ ι α} [a.simple] {x : σ₁} {y : σ₂}
+  (h₁ : a.valid x) (h₂ : b.valid y) (H : b.to_order y ≤ a.to_order x) (n : ℕ) :
+  a.eval_steps n (a.next x h₁) * b.eval₀ y h₂ = 0 :=
+by { rw [finsupp.mul_eq_zero_of_disjoint_support], exact (Stream.mul_eq_zero_aux h₂ h₁ H n).symm, }
+
+end lemmas
+
+example {P Q : Prop} : (¬P ∨ Q) ↔ (P → Q) := imp_iff_not_or.symm
+
+theorem Stream.mul_spec_aux (a : Stream σ₁ ι α) (b : Stream σ₂ ι α) [a.simple] [b.simple] (n : ℕ)
+  {x y B₁ B₂} (ha : a.bound_valid B₁ x) (hb : b.bound_valid B₂ y) (hn : n = B₁ + B₂) :
+  ∃ (k₁ k₂ : ℕ), k₁ ≤ B₁ ∧ k₂ ≤ B₂ ∧ n = k₁ + k₂ ∧ 
+    (a ⋆ b).eval_steps n (x, y) = (a.eval_steps k₁ x) * (b.eval_steps k₂ y) ∧
+    ((a ⋆ b).valid ((a ⋆ b).next'^[n] (x, y)) → ((a ⋆ b).next'^[n] (x, y)) = (a.next'^[k₁] x, b.next'^[k₂] y)) :=
+begin
+  induction n with n ih generalizing B₁ B₂ x y,
+  { use [0, 0], simp, },
+  by_cases H : (a ⋆ b).valid (x, y), swap,
+  { simp only [Stream.eval_invalid H, Stream.next'_val_invalid' H],
+    refine ⟨B₁, B₂, rfl.le, rfl.le, hn, _, false.elim ∘ H⟩,
+    cases (show ¬a.valid x ∨ ¬b.valid y, by simpa [not_and_distrib] using H) with h;
+    simp [Stream.eval_invalid h], },
+  cases B₁, { cases H.1.bound_pos ha, },
+  cases B₂, { cases H.2.bound_pos hb, },
+  simp [nat.succ_eq_add_one, ← add_assoc] at hn,
+  by_cases h : a.to_order x ≤ b.to_order y,
+  { -- Advance `a` (i.e. `a ≤ b`)
+    rw [Stream.bound_valid_succ] at ha,
+    obtain ⟨k₁, k₂, hk₁, hk₂, rfl, he, hiter⟩ := ih (ha H.1) hb (hn.trans (add_right_comm _ _ _)),
+    refine ⟨k₁ + 1, k₂, nat.succ_le_succ hk₁, hk₂, (add_right_comm k₁ k₂ 1), _, _⟩,
+    { simp [H, H.1, h, he, add_mul], congr, 
+      cases k₂, { exfalso, linarith only [hn, hk₁], },
+      simp [H.2, mul_add, Stream.mul_eq_zero H.1 H.2 h, Stream.mul_eval₀], },
+    simp only [Stream.next'_val H, function.iterate_succ_apply, Stream.mul_next, h, if_true, Stream.next'_val H.1],
+    exact hiter, },
+  { -- Advance `b` (i.e. `b < a`)
+    push_neg at h,
+    rw [Stream.bound_valid_succ] at hb,
+    obtain ⟨k₁, k₂, hk₁, hk₂, rfl, he, hiter⟩ := ih ha (hb H.2) hn,
+    refine ⟨k₁, k₂ + 1, hk₁, nat.succ_le_succ  hk₂, rfl, _, _⟩,
+    { simp [H, H.2, h.not_le, he, mul_add], congr,
+      cases k₁, { exfalso, linarith only [hn, hk₂], },
+      simp [H.1, add_mul, Stream.mul_eval₀, Stream.mul_eq_zero' H.1 H.2 h.le], },
+    simp only [Stream.next'_val H, function.iterate_succ_apply, Stream.mul_next, h.not_le, if_false, Stream.next'_val H.2],
+    exact hiter, }
+end
+
+lemma Stream.mul_spec (a : Stream σ₁ ι α) (b : Stream σ₂ ι α) [a.simple] [b.simple]
+  {x y B₁ B₂} (ha : a.bound_valid B₁ x) (hb : b.bound_valid B₂ y) :
+  (a ⋆ b).eval_steps (B₁ + B₂) (x, y) = (a.eval_steps B₁ x) * (b.eval_steps B₂ y) ∧ 
+  ((a ⋆ b).valid ((a ⋆ b).next'^[B₁ + B₂] (x, y)) → ((a ⋆ b).next'^[B₁ + B₂] (x, y) = (a.next'^[B₁] x, b.next'^[B₂] y))) :=
+begin
+  obtain ⟨k₁, k₂, hk₁, hk₂, hs, he, hiter⟩ := Stream.mul_spec_aux a b (B₁ + B₂) ha hb rfl,
+  obtain ⟨rfl, rfl⟩ : k₁ = B₁ ∧ k₂ = B₂ := by split; linarith only [hk₁, hk₂, hs],
+  exact ⟨he, hiter⟩,
+end
 
 @[simps]
-def StreamExec.mul {σ₁ σ₂} (a : StreamExec σ₁ ι α) (b : StreamExec σ₂ ι α) : StreamExec (σ₁ × σ₂) ι α :=
-{ stream := a.stream.mul b.stream,
+def StreamExec.mul (a : StreamExec σ₁ ι α) (b : StreamExec σ₂ ι α) : StreamExec (σ₁ × σ₂) ι α :=
+{ stream := a.stream ⋆ b.stream,
   state := (a.state, b.state),
   bound := a.bound + b.bound }
 
-infix ` ⋆ `:71 := StreamExec.mul
+infixl ` ⋆ `:71 := StreamExec.mul
 
-open StreamExec
 
-@[simp] lemma StreamExec.mul.valid (a : StreamExec σ₁ ι α) (b : StreamExec σ₂ ι α) : (a ⋆ b).valid ↔ a.valid ∧ b.valid := iff.rfl.
-
-lemma Stream.mul.valid.comm (a : Stream σ₁ ι α) (b : Stream σ₂ ι α) (s₁ s₂) :
-  (a.mul b).valid (s₁, s₂) ↔ (b.mul a).valid (s₂, s₁) := by simp [and.comm].
-
-lemma StreamExec.mul.valid.comm (a : StreamExec σ₁ ι α) (b : StreamExec σ₂ ι α) :
-  (a ⋆ b).valid ↔ (b ⋆ a).valid := Stream.mul.valid.comm _ _ _ _.
-
-lemma Stream.mul.ready.comm (a : Stream σ₁ ι α) (b : Stream σ₂ ι α) (s₁ s₂) :
-  Stream.mul.ready a b (s₁, s₂) ↔ Stream.mul.ready b a (s₂, s₁) := begin
-  simp [Stream.mul.ready_iff, and_comm, eq_comm],
-end
-
-lemma StreamExec.mul.ready.comm (a : StreamExec σ₁ ι α) (b : StreamExec σ₂ ι α) :
-  (a ⋆ b).ready ↔ (b ⋆ a).ready := Stream.mul.ready.comm _ _ _ _.
-
-lemma Stream.mul.index.comm (a : Stream σ₁ ι α) (b : Stream σ₂ ι α) (s₁ s₂)
-  (h : (a.mul b).valid (s₁, s₂)) (h' : (b.mul a).valid (s₂, s₁)) :
-  (a.mul b).index (s₁, s₂) h = (b.mul a).index (s₂, s₁) h' :=
-  by simpa [Stream.mul] using max_comm _ _.
-
-lemma StreamState.mul.now'.index.comm {a : Stream σ₁ ι α} {b : Stream σ₂ ι α} :
-  (StreamState.mk (a.mul b) (s₁, s₂)).now'.index =
-  (StreamState.mk (b.mul a) (s₂, s₁)).now'.index := begin
-
-  simp only [StreamState.now'],
-  split_ifs,
-  { simp [max_comm] },
-  { simp at h h_1, exact absurd h.1 (h_1 h.2) },
-  { simp at h h_1, exact absurd h_1.1 (h h_1.2) },
-  { refl }
-end
-
-lemma mul.to_order_tuple.comm (a : Stream σ₁ ι α) (b : Stream σ₂ ι α) (s₁ : σ₁) (s₂ : σ₂) :
-  { StreamState . stream := a.mul b, state := (s₁, s₂) }.to_order_tuple =
-  { StreamState . stream := b.mul a, state := (s₂, s₁) }.to_order_tuple := begin
-
-  simp only [StreamState.to_order_tuple, prod.mk.inj_iff],
-  split,
-  { simp_rw [StreamState.now', Stream.mul.valid.comm] },
-  split,
-  { exact StreamState.mul.now'.index.comm _ _ },
-  { simp_rw [StreamState.now', Stream.mul_ready, Stream.mul.ready.comm] }
-end
-
-lemma mul.invalid (a : StreamExec σ₁ ι α) (b : StreamExec σ₂ ι α) :
-¬ a.valid ∨ ¬ b.valid → ¬ (a.mul b).valid := λ d,
+lemma StreamExec.mul_bound_valid (a : StreamExec σ₁ ι α) (b : StreamExec σ₂ ι α) [a.stream.simple] [b.stream.simple]
+  (ha : a.bound_valid) (hb : b.bound_valid) :
+  (a ⋆ b).bound_valid :=
 begin
-  cases d;
-  simp [d],
+  rw [StreamExec.bound_valid, bound_valid_iff_next'_iterate],
+  intro H,
+  have := (Stream.mul_spec _ _ ha hb).2 H,
+  simp [this] at H,
+  rw [StreamExec.bound_valid, bound_valid_iff_next'_iterate] at ha,
+  exact absurd H.1 ha,
 end
 
-def Stream.reduced' (q : Stream σ ι α) : Prop :=
-∀ {s t} (hs : q.valid s) (ht : q.valid t), q.ready s → q.ready t → q.index s hs = q.index t ht → s = t
-
-class Stream.is_simple (q : Stream σ ι ρ) : Prop :=
-(monotonic : ∀ {r} (h : q.valid r), StreamState.lag ⟨q, r⟩ ⟨q, q.next r h⟩)
-(reduced : ∀ {s t} (hs : q.valid s) (ht : q.valid t), q.ready s → q.ready t → q.index s hs = q.index t ht → s = t)
-
-@[simp] def StreamExec.is_simple : Prop := q.stream.is_simple
-
-@[simps]
-def StreamExec.succ : StreamExec σ ι ρ :=
-{ stream := q.stream,
-  state := if h : q.valid then q.stream.next q.state h else q.state,
-  bound := q.bound.pred }
-
-@[simp] def StreamExec.succ.stream : q.succ.stream = q.stream := rfl
-
-open StreamExec
-
-@[simp] lemma delta_stream_eq (h : a.valid) : (a.δ h).stream = a.stream := rfl
-@[simp] lemma succ_stream_eq : a.succ.stream = a.stream := rfl
-@[simp] lemma succ_bound : a.succ.bound = a.bound.pred := rfl
-
-@[simp] lemma delta_succ (h : q.valid) : q.δ h = q.succ :=
-begin
-  simp only [succ],
-  split_ifs,
-  refl,
-end
-
-variables {a b}
-lemma invalid_succ_invalid : ¬ a.valid → ¬ a.succ.valid :=
-λ h v, begin simp only [succ] at v, split_ifs at v, exact h v end
-
-@[simp] lemma invalid_succ_eq : ¬ a.valid → a.succ.valid = ff :=
-λ h, begin simp [succ], split_ifs, simp [StreamExec.valid], simpa using h end
-
-lemma succ_bound_valid' {s : Stream σ ι α} {σ₀ : σ} {n : ℕ} (h : s.bound_valid n σ₀)
-  (hv : s.valid σ₀) : s.bound_valid (n - 1) (s.next σ₀ hv) :=
-by { induction h, { trivial, }, assumption, }
-
-lemma succ_bound_valid (h : a.bound_valid) : a.succ.bound_valid :=
-begin
-  simp [StreamExec.bound_valid] at *,
-  split_ifs with H,
-  { exact succ_bound_valid' h H, },
-  { exact Stream.bound_valid.start _ H, },
-end
-
-lemma lag.lt_iff_le_not_le : a ⊏ b ↔ (a ⊑ b ∧ ¬ b ⊑ a) := begin
-split,
-intro h,
-split,
-{ exact le_of_lt h },
-{ simpa [StreamExec.lag, StreamExec.lag_lt, le_of_lt] using h },
-{ simp [StreamExec.lag, StreamExec.lag_lt, le_of_lt] },
-end
-
-@[simp] lemma le_succ_left (v : (a ⋆ b).valid) : a.bound_valid → b.bound_valid → a ⊑ b → (a ⋆ b).succ = a.succ ⋆ b :=
-begin
-  intros ha _ le,
-  simp at v,
-  have : a.valid := v.1,
-  have : a.bound ≠ 0,
-  { intro,
-    simpa [StreamExec.bound_valid, *] using ha },
-  obtain ⟨_, _⟩ := nat.exists_eq_succ_of_ne_zero this,
-
-  simp [StreamExec.succ],
-  split_ifs,
-  simp [nat.succ_add, nat.pred, (⋆), *],
-end
-@[simp] lemma lt_succ_right (v : (a ⋆ b).valid) : a.bound_valid → b.bound_valid → b ⊏ a → (a ⋆ b).succ = a ⋆ b.succ :=
-begin
-  intros _ hb lt,
-  simp at v,
-  have : b.valid := v.2,
-  have : ¬ a ⊑ b, { simp only [lag.lt_iff_le_not_le] at lt, simp [lt], },
-  have : b.bound ≠ 0,
-  { intro, simpa [StreamExec.bound_valid, *] using hb },
-    obtain ⟨_, _⟩ := nat.exists_eq_succ_of_ne_zero this,
-
-  simp [StreamExec.succ],
-  split_ifs,
-  simp [nat.add_succ, nat.pred, (⋆), *],
-end
-
-variables (a b)
-
-lemma mul.bound_valid
-(a : StreamExec σ₁ ι α) (b : StreamExec σ₂ ι α) :
-a.bound_valid → b.bound_valid → (a.mul b).bound_valid :=
-begin
-  intros h1 h2,
-  generalize ha : a.bound = n₁,
-  generalize hb : b.bound = n₂,
-  induction n₁ with _ _ c d e f g h generalizing a n₂ b;
-  induction n₂ with _ _ k l m n o p generalizing b,
-  { apply bound_valid.start, simp [StreamExec.bound_valid, *] at * },
-  { apply bound_valid.start, simp [StreamExec.bound_valid, *] at * },
-  { apply bound_valid.start, simp [StreamExec.bound_valid, *] at * },
-  {
-    cases em a.valid; cases em b.valid,
-    { simp only [StreamExec.mul_bound, StreamExec.bound_valid, *],
-      have : (a ⋆ b).valid, { simp, split; assumption },
-      apply bound_valid.step this,
-      simp only [delta_succ],
-      cases em (a ⊑ b) with ale nale,
-      { rw le_succ_left,
-        change bound_valid (n₁_n.succ + n₂_n) (a.succ ⋆ b),
-        rw [nat.succ_add],
-        have ha' : a.succ.bound = n₁_n, { simp [succ, *] },
-        rw [← ha', ← nat.add_succ, ← hb],
-        change (a.succ ⋆ b).bound_valid,
-        have := succ_bound_valid h1,
-        apply n₁_ih,
-        all_goals { assumption },
-      },
-
-      cases le_total a b with le le, {contradiction},
-      { have : b ⊏ a,
-        { rw lag.lt_iff_le_not_le,
-          simp [*] },
-        simp only [lt_succ_right, *],
-        have hb' : b.succ.bound = n₂_n, { simp [succ, *] },
-        rw [← hb', ← ha],
-        change (a ⋆ b.succ).bound_valid,
-        apply n₂_ih,
-        { exact succ_bound_valid h2 },
-        { assumption }
-      },
-    },
-    { apply bound_valid.start, simp [StreamExec.valid, *] at * },
-    { apply bound_valid.start, simp [StreamExec.valid, *] at * },
-    { apply bound_valid.start, simp [StreamExec.valid, *] at * } }
-end
-
-lemma prod_le_iff {α₁ β₁} [has_lt α₁] [has_le β₁] (a b : α₁ ×ₗ β₁) :
-  a ≤ b ↔
-    a.1 < b.1 ∨
-    a.1 = b.1 ∧ a.2 ≤ b.2 := prod.lex_def _ _
-
-lemma bool_not_iff (a b : bool) : !a = !b ↔ a = b :=
-  by cases a; cases b; simp
-
-lemma mul.mono.a_lags_b {a : Stream σ₁ ι α} {b : Stream σ₂ ι α}
-  [ha : a.is_simple] [hb : b.is_simple]
-  {r} (h : (a.mul b).valid r) :
-  (StreamState.mk a r.1) ⊑ₛ (StreamState.mk b r.2) →
-  (StreamState.mk (a.mul b) r) ⊑ₛ (StreamState.mk (a.mul b) (a.next r.1 h.1, r.2)) := begin
-
-  intro a_lags,
-  cases h with ha_valid hb_valid,
-  let r' := (a.next r.fst _, r.snd),
-  have a_mono := is_simple.monotonic ha_valid,
-  simp only [StreamState.lag, StreamState.to_order_tuple, StreamState.now', bool_not_iff] at ⊢ a_mono a_lags,
-
-  rw prod_le_iff at a_lags,
-  cases a_lags with ab_valid_lt a_lags,
-  { -- a is valid but b is invalid (impossible case)
-    revert ab_valid_lt,
-    simp only [bool.lt_iff, bool.of_to_bool_iff, to_bool_iff, and_imp],
-    intros _ hb_invalid, from absurd hb_valid hb_invalid
-  },
-
-  rw prod_le_iff at a_mono,
-  cases a_mono with valid_lt hh,
-  { -- a went from valid to invalid
-    left, simpa only [hb_valid, Stream.mul_valid, and_true] using valid_lt
-  },
-
-  cases hh with valid_eq hh,
-  replace valid_eq : a.valid r.fst ↔ a.valid (a.next r.fst ha_valid) :=
-    by simpa only [bool_not_iff, bool.of_to_bool_iff, bool.to_bool_not, bool.to_bool_eq] using valid_eq,
-
-  have ha_valid' : a.valid (a.next r.fst _) := valid_eq.mp ha_valid,
-
-  rw prod_le_iff at |- hh,
-  right, rw prod_le_iff,
-
-  split,
-  { -- Since a's validity did not change,
-    -- (a.mul b)'s validity must not change either.
-    simp only [bool.of_to_bool_iff, bool.to_bool_eq, not_iff_not],
-
-    change (a.mul b).valid r ↔ (a.mul b).valid r',
-      simp only [Stream.mul_valid],
-      split; rw and_imp; intros _ h; split; assumption'
-  },
-
-  cases hh with idx_lt hh,
-  { -- a's index increased
-    rw prod_le_iff at a_lags,
-    split_ifs at ⊢ idx_lt,
-    { -- a and b remain valid.
-      rw with_top.coe_eq_coe at ⊢,
-      rw with_top.coe_lt_coe at ⊢ idx_lt,
-      cases em (b.index r.snd _ < a.index (a.next r.fst _) _) with idx'_gt idx'_le,
-      { -- a's new index > b's
-        left,
-        show (a.mul b).index r _ < (a.mul b).index r' _,
-          simp only [Stream.mul_index, with_top.coe_lt_coe, max_lt_iff],
-          split; apply lt_max_iff.mpr; left; assumption
-      },
-      { -- a's new index ≤ b's
-        right,
-        simp only [not_lt] at idx'_le,
-        simp only [bool.le_iff_imp, bool.of_to_bool_iff],
-        split,
-
-        show (a.mul b).index r _ = (a.mul b).index r' _,
-          simp only [Stream.mul_index, with_top.coe_eq_coe],
-          rw max_eq_right idx'_le,
-          rw max_eq_right (has_le.le.trans (le_of_lt idx_lt) idx'_le),
-
-        show (a.mul b).ready r → (a.mul b).ready r',
-          suffices : ¬(a.mul b).ready r,
-            intro h, from absurd h this,
-          simp only [Stream.mul_ready],
-          have : a.index r.fst _ < b.index r.snd _ :=
-            has_lt.lt.trans_le idx_lt idx'_le,
-          intro h, from absurd h.index (ne_of_lt this),
-      }
-    },
-
-    -- Various impossible cases (either a or b is invalid).
-    all_goals {
-      { simp only [Stream.mul_index, Stream.mul_valid, not_and] at h_1,
-        from absurd hb_valid (h_1 ha_valid') }
-      <|>
-      { simp only [Stream.mul_index, Stream.mul_valid, not_and] at h,
-        from absurd hb_valid (h ha_valid) }
-      <|>
-      contradiction
-    }
-  },
-
-  right,
-  cases hh with idx_eq ready_le,
-  { -- a became ready or stayed the same
-    simp only [bool_not_iff, bool.le_iff_imp, bool.of_to_bool_iff] at ⊢ idx_eq ready_le,
-    split_ifs at ⊢ idx_eq ready_le,
-    { -- a and b remain valid
-      rw with_top.coe_eq_coe at ⊢ idx_eq,
-      split,
-      show (a.mul b).index r _ = (a.mul b).index r' _,
-        simp only [Stream.mul_index, idx_eq],
-
-      show (a.mul b).ready r → (a.mul b).ready r',
-        simp only [Stream.mul_ready],
-        intro prev_mul_ready,
-        cases prev_mul_ready.ready with ha_ready hb_ready,
-
-        have ha_ready' : a.ready (a.next r.fst _) := ready_le ha_ready,
-        exact {
-          valid := ⟨ha_valid', hb_valid⟩,
-          ready := ⟨ha_ready', hb_ready⟩,
-          index := begin
-            have := prev_mul_ready.index,
-            transitivity; { symmetry, assumption } <|> assumption
-          end,
-        }
-    },
-
-    -- Various impossible cases (either a or b is invalid).
-    all_goals {
-      { simp only [Stream.mul_index, Stream.mul_valid, not_and] at h_1,
-        from absurd hb_valid (h_1 ha_valid') }
-      <|>
-      { simp only [Stream.mul_index, Stream.mul_valid, not_and] at h,
-        from absurd hb_valid (h ha_valid) }
-      <|>
-      contradiction
-    }
-  }
-end
-
-instance hmul.is_simple
-(a : Stream σ₁ ι α) (b : Stream σ₂ ι α)
-[ha : a.is_simple] [hb : b.is_simple] : (a.mul b).is_simple :=
-{ monotonic := begin
-    intros r h,
-    obtain ⟨s₁, s₂⟩ := r,
-    obtain ⟨ha_valid, hb_valid⟩ := h,
-    rw Stream.mul_next,
-
-    split_ifs with lags,
-    { -- a lags b
-      apply mul.mono.a_lags_b, refine ⟨ha_valid, hb_valid⟩, assumption },
-
-    { -- b (strictly) lags a; weaken the hypothesis first to reuse mul.mono.a_lags_b
-      have := le_of_lt (not_le.mp lags),
-      simp_rw [StreamState.lag, mul.to_order_tuple.comm a b],
-      apply mul.mono.a_lags_b,
-      { exact ⟨hb_valid, ha_valid⟩ },
-      { assumption }
-    }
-  end,
-
-  reduced :=
-  begin
-    intros s t hs ht ready_s ready_t eq,
-    cases ready_s,
-    cases ready_t,
-
-    simp only [(*), Stream.mul] at hs ht,
-    simp [Stream.mul, *, max_idem.idempotent] at eq,
-
-    ext,
-    { apply @is_simple.reduced _ _ _ _ _ ha; simp [*] },
-    { apply @is_simple.reduced _ _ _ _ _ hb; simp [*] },
-  end
-}
-
-#check primitives.range 2
-
-instance primitives.range.is_simple (n : ℕ) : (primitives.range n).is_simple := {
-  monotonic := begin
-    intros ctr h_valid,
-    simp only [StreamState.lag, StreamState.to_order_tuple, StreamState.now', prod_le_iff],
-    cases em (n ≤ ctr + 1),
-    { left,
-      simp only [primitives.range] at ⊢ h_valid,
-      simp only [bool.lt_iff],
-      split; simpa },
-    { right, split,
-      { simp only [primitives.range] at ⊢ h_valid,
-        simp [h_valid, lt_of_not_le h] },
-      { left, split_ifs,
-        { simp [with_top.coe_lt_coe, primitives.range] },
-        { apply with_top.coe_lt_top },
-        { contradiction },
-        { apply with_top.coe_lt_top } } }
-  end,
-
-  reduced := begin
-    intros s t hs ht ready_s ready_t eq,
-    cases ready_s,
-    cases ready_t,
-
-    simp only [primitives.range] at eq,
-    assumption
-  end,
-}
-
-example : (primitives.range 2).is_simple := infer_instance
-example : ((primitives.range 2).mul (primitives.range 3)).is_simple := by apply_instance
-example : (((primitives.range 2).mul (primitives.range 3)).mul (primitives.range 4)).is_simple := by apply_instance
-
-variables
-(a_simple : a.is_simple)
-(b_simple : b.is_simple)
-
-def StreamExec.eval₀' [has_zero α] (s : StreamExec σ ι α) : ι →₀ α :=
-if h : s.valid ∧ s.ready then finsupp.single (s.now h.1 h.2).index (s.now h.1 h.2).value else 0
-
-noncomputable def StreamExec.eval_steps' [add_zero_class α] :
-  ℕ → (StreamExec σ ι α) → ι →₀ α
-| 0 s := 0
-| (n + 1) s := (StreamExec.eval_steps' n (s.succ)) + (s.eval₀')
-
-@[simp]
-def StreamExec.eval' [add_zero_class α] (s : StreamExec σ ι α) : ι →₀ α :=
-s.eval_steps' s.bound
-
-open StreamExec
-
-@[simp] lemma not_ready_eval₀_zero : ¬ s.ready → s.eval₀' = 0 :=
-begin
-  intro n,
-  simp [eval₀', n],
-end
-
-@[simp] lemma not_ready_mul_eval₀_zero_l : ¬ a.ready → (a ⋆ b).eval₀' = 0 :=
-begin
-  intro n,
-  simp [eval₀'],
-  rintro ⟨_, ⟨_, ⟨_,_⟩, _⟩⟩, contradiction,
-end
-
-@[simp] lemma not_ready_mul_eval₀_zero_r : ¬ b.ready → (a ⋆ b).eval₀' = 0 :=
-begin
-  intro n,
-  simp [eval₀'],
-  rintro ⟨_, ⟨_, ⟨_,_⟩, _⟩⟩, contradiction,
-end
-
-@[simp] lemma invalid_eval₀_zero : ¬ a.valid → a.eval₀' = 0 := begin simp [eval₀'], rintro _ ⟨_, _⟩, contradiction end
-
-@[simp] lemma invalid_zero {n} : ¬ a.valid → a.eval_steps' n = 0 := begin
-  intros h,
-  induction n generalizing a,
-  { simp [eval_steps'] },
-  { have : ¬ a.succ.valid := invalid_succ_invalid h, simp [eval_steps', *] },
-end
-
-@[simp] lemma invalid_mul_zero_l {n} : ¬ a.valid → (a ⋆ b).eval_steps' n = 0 :=
-begin
-  intros h,
-  have : ¬ (a ⋆ b).valid, { simp [h] },
-  induction n generalizing a,
-  { simp [eval_steps'] },
-  { have : ¬ (a ⋆ b).succ.valid := invalid_succ_invalid this, simp [eval_steps', *] },
-end
-@[simp] lemma invalid_mul_zero_r {n} : ¬ b.valid → (a ⋆ b).eval_steps' n = 0 :=
-begin
-  intros h,
-  have : ¬ (a ⋆ b).valid, { simp [h] },
-  induction n generalizing a,
-  { simp [eval_steps'] },
-  { have : ¬ (a ⋆ b).succ.valid := invalid_succ_invalid this, simp [eval_steps', *] },
-end
-@[simp] lemma invalid_eval₀_zero_l : ¬ a.valid → (a ⋆ b).eval₀' = 0 :=
-begin
-  intros h,
-  have : ¬ (a ⋆ b).valid, { simp [h] },
-  simp [eval₀'],
-  rintros ⟨_, _⟩,
-  contradiction,
-end
-@[simp] lemma invalid_eval₀_zero_r : ¬ b.valid → (a ⋆ b).eval₀' = 0 :=
-begin
-  intros h,
-  have : ¬ (a ⋆ b).valid, { simp [h] },
-  simp [eval₀'],
-  rintros ⟨_, _⟩,
-  contradiction,
-end
-
-@[simp] lemma eval_steps_zero' : eval_steps' 0 a = 0 := rfl
-
-@[simp] lemma not_bool_eq : ∀ {a b : bool}, !a = !b ↔ a = b := by { intros, cases a; cases b; dec_trivial }
-
-@[simp] lemma StreamState.order_eq_iff (a : StreamState σ₁ ι α) (b : StreamState σ₁ ι β) :
-a.to_order_tuple = b.to_order_tuple ↔
-a.valid = b.valid ∧ a.now'.index = b.now'.index ∧ a.ready = b.ready :=
-by { simp [StreamState.to_order_tuple, StreamState.now'], }
-
-@[simp] lemma StreamState.simp_ext : ({stream := a.to_StreamState.stream, state := a.to_StreamState.state} : StreamState σ₁ ι α) = a.to_StreamState := StreamState.ext _ a.to_StreamState rfl rfl
-
-variable
-(ss : StreamState σ ι ρ)
-
-lemma succ_state_not_eq (h : a.valid) (bv : a.bound_valid) : a.state ≠ a.succ.state :=
-begin
-  simp [bound_valid] at bv,
-  induction bv,
-  { contradiction },
-  { intro eq,
-    set eq := eq.symm,
-    simp at eq,
-    simp [eq h] at bv_ih,
-    apply bv_ih,
-    simp [succ],
-    split_ifs,
-    simpa [StreamExec.valid, h, eq] using bv_h }
-end
-
-@[simp] theorem with_top_inj {a b : ι} : (↑ a : with_top ι) = ↑ b ↔ a = b :=
-by { simp [← with_top.some_eq_coe, option.some_inj] }
-
-lemma reduced_ready_progress (h : a.valid) (bv : a.bound_valid) : a.stream.is_simple → a.ready → a ⊏ a.succ :=
-begin
-  intros as ar,
-  cases as with mono red,
-  have := mono h,
-  simp [StreamState.lag, le_iff_eq_or_lt] at this,
-  cases this,
-  { obtain ⟨eqv, eqi, eqr⟩ := this,
-    suffices : a.state = a.succ.state,
-    { have := succ_state_not_eq a h bv, contradiction },
-    { have : a.stream.valid (a.to_StreamState.stream.next a.to_StreamState.state h),
-      { apply eqv.mp, assumption },
-      simp [succ], split_ifs,
-
-      apply red h this,
-      { assumption, },
-      { apply eqr.mp, assumption },
-      { simp [StreamExec.valid] at h,
-        simp [StreamState.now'] at eqi,
-        simp [StreamState.valid] at eqv,
-
-        split_ifs at eqi,
-        simpa using eqi } } },
-  { simp [StreamExec.to_order_tuple, StreamExec.lag_lt, succ, *] },
-end
-
-@[simp] lemma is_simple_succ_is_simple : q.succ.is_simple ↔ q.is_simple := iff.rfl
-
-section algebra
-open StreamState
-
-@[simp] lemma lt_mul_eval₀ : a ⊏ b → a.eval₀' * b.eval₀' = 0 :=
-begin
-intro lt,
-simp [eval₀'],
-split_ifs with ha hb,
-{ suffices : a.to_StreamState.stream.index a.to_StreamState.state ha.1 ≠ b.to_StreamState.stream.index b.to_StreamState.state hb.1,
-  { ext,
-    rw finsupp.mul_apply,
-    simp [finsupp.single],
-    intros e1 e2, simp [e1, e2] at this,
-    contradiction },
-  {
-    intro eq,
-    have := ha.1,
-    have := ha.2,
-    have := hb.1,
-    have := hb.2,
-    simp [StreamExec.valid, StreamExec.ready] at *,
-    simp [StreamExec.lag_lt, StreamExec.to_order_tuple, StreamState.to_order_tuple, StreamState.now'] at lt,
-    simp [to_bool_tt, *] at lt,
-    exact lt
-  }
-},
-{ simp },
-{ simp },
-{ simp },
-end
-
-@[simp] lemma lt_mul_eval₀_r : b ⊏ a → a.eval₀' * b.eval₀' = 0 :=
-begin
-intro lt,
-simp [eval₀'],
-split_ifs with ha hb,
-{ suffices : a.to_StreamState.stream.index a.to_StreamState.state ha.1 ≠ b.to_StreamState.stream.index b.to_StreamState.state hb.1,
-  { ext,
-    rw finsupp.mul_apply,
-    simp [finsupp.single],
-    intros e1 e2, simp [e1, e2] at this,
-    contradiction },
-  {
-    intro eq,
-    have := ha.1,
-    have := ha.2,
-    have := hb.1,
-    have := hb.2,
-    simp [StreamExec.valid, StreamExec.ready] at *,
-    simp [StreamExec.lag_lt, StreamExec.to_order_tuple, StreamState.to_order_tuple, StreamState.now'] at lt,
-    simp [to_bool_tt, *] at lt,
-    exact lt
-  }
-},
-{ simp },
-{ simp },
-{ simp },
-end
-
-variables {a}
-lemma succ_squb : a.is_simple → a ⊑ a.succ := begin
-intro h,
-cases h with mono _,
-cases em a.valid with h h,
-{ simp only [*, succ],
-  exact mono h },
-{ simp only [*, succ],
-  change a≤a,
-  refl }
-end
-variables (a)
-
-@[simp] lemma lt_mul_eval {n} (hb : b.is_simple) :
-a ⊏ b → a.eval₀' * b.eval_steps' n = 0 :=
-begin
-  intro lt,
-  unfreezingI { induction n generalizing b },
-  { simp [*] },
-  simp [eval_steps', left_distrib, *],
-  apply n_ih,
-  { simpa [*] },
-  { exact lt_of_lt_of_le lt (succ_squb hb) }
-end
-
-@[simp] lemma lt_mul_eval_r {n} (ha : a.is_simple) :
-b ⊏ a → a.eval_steps' n * b.eval₀' = 0 :=
-begin
-  intro lt,
-  unfreezingI { induction n generalizing a },
-  { simp [*] },
-  simp [eval_steps', right_distrib, *],
-  apply n_ih,
-  { simpa [*] },
-  { exact lt_of_lt_of_le lt (succ_squb ha) }
-end
-
-@[simp] lemma order_eq_ready_iff (h : a.to_order_tuple = b.to_order_tuple) : (a.ready ↔ b.ready) :=
-by simp [StreamExec.to_order_tuple, StreamState.to_order_tuple, StreamExec.ready, StreamState.now', *] at *
-
-@[simp] lemma order_eq_valid_iff (h : a.to_order_tuple = b.to_order_tuple) : (a.valid ↔ b.valid) :=
-by simp [StreamExec.to_order_tuple, StreamState.to_order_tuple, StreamExec.valid, StreamState.now', *] at *
-
--- @[simp] lemma reduced_mul_succ' {n} (ha : a.is_simple) (hb : b.is_simple) (bv : b.bound_valid) :
--- a ⊑ b → a.eval₀' * b.succ.eval_steps' n = 0 := sorry
-
-@[simp] lemma reduced_mul_succ2 {n} (hb : b.is_simple) (bv : b.bound_valid) :
-a ⊑ b → a.eval₀' * b.succ.eval_steps' n = 0 :=
-begin
-  intro le,
-  cases em a.valid with ha ha; cases em a.ready,
-  {
-    { suffices : a ⊏ b.succ,
-      { rw [lt_mul_eval _ _ _ this],
-        { simpa [succ] } },
-      { cases em (a.to_order_tuple = b.to_order_tuple) with eq eq,
-        {
-          apply lt_of_le_of_lt le (reduced_ready_progress _ _ bv hb _),
-          { rw [← order_eq_valid_iff a _ eq], assumption },
-          { rw [← order_eq_ready_iff a _ eq], assumption },
-        },
-        {
-          simp only [StreamExec.lag] at le,
-          simp [le_iff_eq_or_lt] at le,
-          cases le, contradiction,
-          simp only [StreamExec.lag_lt] at |-,
-          apply lt_of_lt_of_le le,
-          apply succ_squb, assumption,
-        },
-      }
-  } },
-  { simp [*] },
-  { simp [*] },
-  { simp [*] },
-
-end.
-
-lemma mul_eval₀ :
-(a ⋆ b).eval₀'  = a.eval₀' * b.eval₀' :=
-begin
-cases em a.valid with ha; cases em b.valid with hb; cases em a.ready; cases em b.ready,
-{ cases em (a.stream.index a.state ha = b.stream.index b.state hb),
-  { have : (a ⋆ b).ready := ⟨⟨ha, hb⟩, ⟨h, h_1⟩, h_2⟩,
-    simp [*, eval₀'],
-    { ext,
-      simp [finsupp.mul_apply, finsupp.single],
-      split_ifs,
-      refl,
-      refl,
-    },
-  },
-  { suffices : ¬ (a ⋆ b).ready,
-    { have : (a ⋆ b).valid := ⟨ha, hb⟩,
-      simp only [*, eval₀'],
-      ext,
-      rw finsupp.mul_apply,
-      simp [finsupp.single],
-      split_ifs with h_3 h_4,
-      rw h_3 at h_2, rw h_4 at h_2, contradiction,
-      refl, refl },
-    rintro ⟨_, _, h⟩, simp [(⋆)] at h, rw h at h_2, contradiction,
-} },
-
-all_goals { simp [*] },
-end
-
-end algebra
-
--- @[simp] lemma reduced_mul_eval_l (ha : a.is_simple) (hb : b.is_simple) (vb : b.bound_valid) :
--- a ⊑ b → (a ⋆ b).eval₀'  = a.eval₀' * b.eval' :=
--- begin
---   intros le,
---   simp,
---   generalize h : b.bound = n,
---   unfreezingI { induction n generalizing b },
---   { simp at h, suffices : ¬ b.valid,
---     { simp [this] },
---     { simpa [bound_valid, h] using vb } },
---   { simp [eval_steps', left_distrib], suffices : a ⊑ b.succ, simp [*],
---     have := succ_squb hb,
---     simp [StreamExec.lag, StreamExec.lag_lt] at le this |-,
---     exact le_trans le this }
--- end
-
-@[simp] lemma reduced_mul_eval_r (ha : a.is_simple) (hb : b.is_simple) (va : a.bound_valid) :
-b ⊏ a → (a ⋆ b).eval₀' = a.eval' * b.eval₀' :=
-begin
-  intros le,
-  simp,
-  generalize h : a.bound = n,
-  unfreezingI { induction n generalizing a },
-  { simp at h, suffices : ¬ a.valid,
-    { simp [this] },
-    { simpa [bound_valid, h] using va } },
-  { simp [eval_steps', right_distrib], suffices : b ⊏ a.succ, simp [*],
-    have := succ_squb ha,
-    simp [StreamExec.lag, StreamExec.lag_lt] at le this |-,
-    exact lt_of_lt_of_le le this }
-end
-
-theorem mul_spec : a.bound_valid → b.bound_valid → a.is_simple → b.is_simple → (a ⋆ b).eval' = a.eval' * b.eval' :=
-begin
-  intros abv bbv _ _,
-  simp,
-  generalize hba : a.bound = ba,
-  generalize hbb : b.bound = bb,
-
-  induction ba generalizing a bb b;
-  induction bb generalizing b, simp [StreamExec.eval_steps'],
-
-  { have : ¬ a.valid, { simpa [hba] using abv }, simp [*] },
-  { have : ¬ b.valid, { simpa [hbb] using bbv }, simp [*] },
-
-  cases em a.valid; cases em b.valid,
-
-  { have hav : (a ⋆ b).valid := ⟨h, h_1⟩,
-    cases em (a ⊑ b) with ale nale,
-    {
-      simp only [nat.succ_add, le_succ_left, eval_steps', *],
-      rw ba_ih,
-      { simp [*, eval_steps', right_distrib, left_distrib, mul_eval₀], abel, },
-      { exact succ_bound_valid abv },
-      { assumption },
-      { simpa },
-      { assumption },
-      { simp [*] },
-      { simp [*] },
-    },
-    cases le_total a b with le le, {contradiction},
-    {
-      have : b ⊏ a,
-      { rw lag.lt_iff_le_not_le,
-        simp [*] },
-
-      simp only [nat.add_succ, lt_succ_right, eval_steps', *],
-      rw bb_ih,
-      { simp [*, eval_steps', right_distrib, left_distrib], },
-      { exact succ_bound_valid bbv },
-      { simpa [*] },
-      { simp [succ, *] },
-    }
-  },
-
-  { have : ¬ (a ⋆ b).valid, {simp [*]}, simp [*] },
-  { have : ¬ (a ⋆ b).valid, {simp [*]}, simp [*] },
-  { have : ¬ (a ⋆ b).valid, {simp [*]}, simp [*] },
-
-end
+@[simp] lemma StreamExec.mul_spec (a : StreamExec σ₁ ι α) (b : StreamExec σ₂ ι α) [a.stream.simple] [b.stream.simple] 
+  (ha : a.bound_valid) (hb : b.bound_valid) :
+  (a ⋆ b).eval = a.eval * b.eval :=  (Stream.mul_spec _ _ ha hb).1
